src/proof/algebra/constrained_gset.v
@@ -1,0 +1,223 @@
+From New.proof Require Import prelude.
+From iris.algebra Require Import cmra gset view.
+From iris.base_logic.lib Require Import own.
+
+(* A linear ghost set whose authoritative set is constrained by [P]. Fragments
+   own individual elements, imply membership in the authoritative set, and can be
+   consumed to remove that element from the authoritative set. *)
+Section constrained_gset.
+Context {K : Type} `{Countable K}.
+Context (P : K → Prop).
+
+Definition authO : ofe := gsetO (leibnizO K).
+Definition fragUR : ucmra := gset_disjUR K.
+
+Implicit Types (a : authO) (b : fragUR).
+
+Local Definition view_rel_raw (n : nat) a b : Prop :=
+  set_Forall P a ∧ ∃ frag_keys, b = GSet frag_keys ∧ frag_keys ⊆ a.
+
+Local Lemma view_rel_raw_mono n1 n2 a1 a2 b1 b2 :
+  view_rel_raw n1 a1 b1 →
+  a1 ≡{n2}≡ a2 →
+  b2 ≼{n2} b1 →
+  (n2 ≤ n1)%nat →
+  view_rel_raw n2 a2 b2.
+Proof.
+  intros [Hvalid_auth [frag_keys1 [Hb1 Hfrag_in_auth1]]] Ha Hb _.
+  assert (Ha_equiv : a1 ≡ a2).
+  { apply (proj2 (discrete_iff n2 a1 a2)). done. }
+  assert (Ha_elem : ∀ key, key ∈ a1 ↔ key ∈ a2).
+  { exact (proj1 (set_equiv a1 a2) Ha_equiv). }
+  subst b1.
+  apply cmra_discrete_included_iff in Hb.
+  destruct b2 as [frag_keys2|].
+  - split.
+    { intros key Hkey.
+      apply Hvalid_auth.
+      apply Ha_elem.
+      done. }
+    exists frag_keys2. split; [done|].
+    apply gset_disj_included in Hb.
+    intros key Hkey.
+    apply Ha_elem.
+    apply Hfrag_in_auth1.
+    apply Hb.
+    done.
+  - exfalso.
+    destruct Hb as [[extra|] Hop]; simpl in Hop; try done.
+Qed.
+
+Local Lemma view_rel_raw_valid n a b :
+  view_rel_raw n a b → ✓{n} b.
+Proof.
+  intros [_ [frag_keys [-> _]]].
+  done.
+Qed.
+
+Local Lemma view_rel_raw_unit n :
+  ∃ a, view_rel_raw n a ε.
+Proof.
+  exists (∅ : gset K).
+  split.
+  - intros key Hkey. Timeout 10 set_solver.
+  - exists (∅ : gset K). split; [done|].
+    Timeout 10 set_solver.
+Qed.
+
+Canonical Structure view_rel : view_rel authO fragUR :=
+  ViewRel view_rel_raw view_rel_raw_mono
+          view_rel_raw_valid view_rel_raw_unit.
+
+Definition auth dq a : viewR view_rel := ●V{dq} a.
+Definition frag b : viewR view_rel := ◯V b.
+
+Local Notation "●CG a" := (auth 1 a) (at level 20).
+Local Notation "◯CG b" := (frag b) (at level 20).
+
+Class constrained_gsetG Σ :=
+  { #[global] constrained_gset_inG :: inG Σ (viewR view_rel); }.
+
+Definition constrained_gsetΣ :=
+  #[GFunctor (viewR view_rel)].
+
+#[global]
+Instance subG_constrained_gsetG Σ :
+  subG constrained_gsetΣ Σ → constrained_gsetG Σ.
+Proof. solve_inG. Qed.
+
+Context `{!constrained_gsetG Σ}.
+
+Definition own_auth γ (reserved_keys : gset K) : iProp Σ :=
+  own γ (●CG reserved_keys).
+
+Definition own_frag γ (key : K) : iProp Σ :=
+  own γ (◯CG (GSet {[key]})).
+
+Global Instance own_auth_timeless γ reserved_keys :
+  Timeless (own_auth γ reserved_keys).
+Proof. unfold own_auth. apply _. Qed.
+
+Global Instance own_frag_timeless γ key :
+  Timeless (own_frag γ key).
+Proof. unfold own_frag. apply _. Qed.
+
+Lemma init :
+  ⊢ |==> ∃ γ, own_auth γ (∅ : gset K).
+Proof.
+  unfold own_auth.
+  iMod (own_alloc (●CG (∅ : gset K))) as (γ) "Hauth".
+  { apply (proj2 (view_auth_dfrac_valid view_rel 1 (∅ : gset K))).
+    split; [done|].
+    intros n. split.
+    - intros key Hkey. Timeout 10 set_solver.
+    - exists (∅ : gset K). split; [done|].
+      Timeout 10 set_solver.
+  }
+  iModIntro. iExists γ. iExact "Hauth".
+Qed.
+
+Lemma auth_set_Forall {γ reserved_keys} :
+  own_auth γ reserved_keys -∗
+  ⌜ set_Forall P reserved_keys ⌝.
+Proof.
+  unfold own_auth.
+  iIntros "Hauth".
+  iDestruct (own_valid with "Hauth") as "Hvalid".
+  iDestruct (internal_cmra_valid_elim with "Hvalid") as %Hvalid.
+  iPureIntro.
+  pose proof (proj1 (view_auth_dfrac_validN view_rel 0%nat 1 reserved_keys) Hvalid)
+    as [_ Hrel].
+  exact (proj1 Hrel).
+Qed.
+
+Lemma frag_elem_of_auth {γ reserved_keys} key :
+  own_auth γ reserved_keys -∗
+  own_frag γ key -∗
+  ⌜ key ∈ reserved_keys ⌝.
+Proof.
+  unfold own_auth, own_frag.
+  iIntros "Hauth Hfrag".
+  iDestruct (own_valid_2 with "Hauth Hfrag") as "Hvalid".
+  iDestruct (internal_cmra_valid_elim with "Hvalid") as %Hvalid.
+  iPureIntro.
+  pose proof (proj1 (view_both_validN view_rel 0%nat reserved_keys (GSet {[key]})) Hvalid)
+    as [_ [frag_keys [Hfrag_eq Hfrag_in_auth]]].
+  injection Hfrag_eq as <-.
+  apply Hfrag_in_auth.
+  Timeout 10 set_solver.
+Qed.
+
+Lemma frag_pred {γ} key :
+  own_frag γ key -∗
+  ⌜ P key ⌝.
+Proof.
+  unfold own_frag.
+  iIntros "Hfrag".
+  iDestruct (own_valid with "Hfrag") as "Hvalid".
+  iDestruct (internal_cmra_valid_elim with "Hvalid") as %Hvalid.
+  iPureIntro.
+  pose proof (proj1 (view_frag_validN view_rel 0%nat (GSet {[key]})) Hvalid)
+    as [reserved_keys [Hvalid_auth [frag_keys [Hfrag_eq Hfrag_in_auth]]]].
+  injection Hfrag_eq as <-.
+  apply Hvalid_auth.
+  apply Hfrag_in_auth.
+  Timeout 10 set_solver.
+Qed.
+
+Lemma reserve_key_vs {γ reserved_keys} key :
+  key ∉ reserved_keys →
+  P key →
+  own_auth γ reserved_keys ==∗
+    own_auth γ ({[key]} ∪ reserved_keys) ∗
+    own_frag γ key.
+Proof.
+  unfold own_auth, own_frag.
+  iIntros (Hkey_not_reserved Hkey_pred) "Hauth".
+  rewrite -own_op.
+  iApply (own_update with "Hauth").
+  apply view_update_alloc.
+  intros n bf [Hvalid_auth [frag_keys [-> Hfrag_in_auth]]].
+  assert (Hdisj : {[key]} ## frag_keys).
+  {
+    intros key' Hkey' Hfrag.
+    apply elem_of_singleton in Hkey'. subst.
+    apply Hkey_not_reserved.
+    apply Hfrag_in_auth.
+    done.
+  }
+  rewrite (gset_disj_union {[key]} frag_keys Hdisj).
+  split.
+  - intros key' Hkey'.
+    rewrite elem_of_union elem_of_singleton in Hkey'.
+    destruct Hkey' as [->|Hkey']; [done|].
+    apply Hvalid_auth. done.
+  - exists ({[key]} ∪ frag_keys).
+    split; [done|].
+    Timeout 10 set_solver.
+Qed.
+
+Lemma consume_key_vs {γ reserved_keys} key :
+  own_auth γ reserved_keys -∗
+  own_frag γ key ==∗
+    own_auth γ (reserved_keys ∖ {[key]}).
+Proof.
+  unfold own_auth, own_frag.
+  iIntros "Hauth Hfrag".
+  iApply (own_update_2 with "Hauth Hfrag").
+  apply view_update_dealloc.
+  intros n bf [Hvalid_auth [frag_keys [Hop Hfrag_in_auth]]].
+  assert (Hvalid_op : ✓ (GSet {[key]} ⋅ bf)).
+  { rewrite Hop. done. }
+  destruct (gset_disj_valid_inv_l {[key]} bf Hvalid_op)
+    as [other_frag_keys [-> Hdisj]].
+  rewrite (gset_disj_union {[key]} other_frag_keys Hdisj) in Hop.
+  injection Hop as <-.
+  split.
+  - intros key' Hkey'.
+    apply Hvalid_auth. Timeout 10 set_solver.
+  - exists other_frag_keys. split; [done|].
+    Timeout 10 set_solver.
+Qed.
+
+End constrained_gset.
